pulse/ulib/experimental/Steel.SelReference.fsti
@@ -1,0 +1,130 @@
+(*
+   Copyright 2020 Microsoft Research
+
+   Licensed under the Apache License, Version 2.0 (the "License");
+   you may not use this file except in compliance with the License.
+   You may obtain a copy of the License at
+
+       http://www.apache.org/licenses/LICENSE-2.0
+
+   Unless required by applicable law or agreed to in writing, software
+   distributed under the License is distributed on an "AS IS" BASIS,
+   WITHOUT WARRANTIES OR CONDITIONS OF ANY KIND, either express or implied.
+   See the License for the specific language governing permissions and
+   limitations under the License.
+*)
+
+module Steel.SelReference
+
+open Steel.Memory
+open Steel.SelEffect.Atomic
+open Steel.SelEffect
+
+module R = Steel.Reference
+open Steel.FractionalPermission
+
+let ref (a:Type0) : Type0 = R.ref a
+let ptr (#a:Type0) (r:ref a) : slprop u#1 = h_exists (R.pts_to r full_perm)
+
+val ptr_sel (#a:Type0) (r:ref a) : selector a (ptr r)
+
+val ptr_sel_interp (#a:Type0) (r:ref a) (m:mem) : Lemma
+  (requires interp (ptr r) m)
+  (ensures interp (R.pts_to r full_perm (ptr_sel r m)) m)
+
+[@@ __steel_reduce__]
+let vptr' #a r : vprop' =
+  {hp = ptr r;
+   t = a;
+   sel = ptr_sel r}
+
+[@@ __steel_reduce__]
+unfold
+let vptr r = VUnit (vptr' r)
+
+val alloc (#a:Type0) (x:a) : SteelSel (ref a)
+  emp (fun r -> vptr r)
+  (requires fun _ -> True)
+  (ensures fun _ r h1 -> h1 (vptr r) == x /\ not (R.is_null r))
+
+val free (#a:Type0) (r:ref a) : SteelSel unit
+  (vptr r) (fun _ -> emp)
+  (requires fun _ -> True)
+  (ensures fun _ _ _ -> True)
+
+val read (#a:Type0) (r:ref a) : SteelSel a
+  (vptr r) (fun _ -> vptr r)
+  (requires fun _ -> True)
+  (ensures fun h0 x h1 -> h0 (vptr r) == h1 (vptr r) /\ x == h1 (vptr r))
+
+val write (#a:Type0) (r:ref a) (x:a) : SteelSel unit
+  (vptr r) (fun _ -> vptr r)
+  (requires fun _ -> True)
+  (ensures fun _ _ h1 -> x == h1 (vptr r))
+
+val vptr_not_null (#opened: _)
+  (#a: Type)
+  (r: R.ref a)
+: SteelSelGhost unit opened
+    (vptr r)
+    (fun _ -> vptr r)
+    (fun _ -> True)
+    (fun h0 _ h1 ->
+      h1 (vptr r) == h0 (vptr r) /\
+      R.is_null r == false
+    )
+
+
+
+[@@ __steel_reduce__]
+let sel (#a:Type) (#p:vprop) (r:ref a)
+  (h:rmem p{FStar.Tactics.with_tactic selector_tactic (can_be_split p (vptr r) /\ True)})
+  = h (vptr r)
+
+(*** Ghost references ***)
+
+[@@ erasable]
+let ghost_ref (a:Type u#0) : Type u#0 = R.ghost_ref a
+let ghost_ptr (#a: Type0) (r: ghost_ref a) : Tot (slprop u#1) = h_exists (R.ghost_pts_to r full_perm)
+
+val ghost_ptr_sel (#a:Type0) (r:ghost_ref a) : selector a (ghost_ptr r)
+
+val ghost_ptr_sel_interp (#a:Type0) (r:ghost_ref a) (m:mem) : Lemma
+  (requires interp (ghost_ptr r) m)
+  (ensures interp (R.ghost_pts_to r Steel.FractionalPermission.full_perm (ghost_ptr_sel r m)) m)
+
+[@@ __steel_reduce__]
+let ghost_vptr' #a r : vprop' =
+  {hp = ghost_ptr r;
+   t = a;
+   sel = ghost_ptr_sel r}
+
+[@@ __steel_reduce__]
+unfold
+let ghost_vptr r = VUnit (ghost_vptr' r)
+
+val ghost_alloc (#a:Type0) (#opened:inames) (x:Ghost.erased a) : SteelSelGhost (ghost_ref a) opened
+  emp (fun r -> ghost_vptr r)
+  (requires fun _ -> True)
+  (ensures fun _ r h1 -> h1 (ghost_vptr r) == Ghost.reveal x)
+
+val ghost_free (#a:Type0) (#opened:inames) (r:ghost_ref a) : SteelSelGhost unit opened
+  (ghost_vptr r) (fun _ -> emp)
+  (requires fun _ -> True)
+  (ensures fun _ _ _ -> True)
+
+let ghost_read (#a:Type0) (#opened:inames) (r:ghost_ref a) : SteelSelGhost (Ghost.erased a) opened
+  (ghost_vptr r) (fun _ -> ghost_vptr r)
+  (requires fun _ -> True)
+  (ensures fun h0 x h1 -> h0 (ghost_vptr r) == h1 (ghost_vptr r) /\ Ghost.reveal x == h1 (ghost_vptr r))
+= gget (ghost_vptr r)
+
+val ghost_write (#a:Type0) (#opened:inames) (r:ghost_ref a) (x:Ghost.erased a) : SteelSelGhost unit opened
+  (ghost_vptr r) (fun _ -> ghost_vptr r)
+  (requires fun _ -> True)
+  (ensures fun _ _ h1 -> Ghost.reveal x == h1 (ghost_vptr r))
+
+[@@ __steel_reduce__]
+let ghost_sel (#a:Type) (#p:vprop) (r:ghost_ref a)
+  (h:rmem p{FStar.Tactics.with_tactic selector_tactic (can_be_split p (ghost_vptr r) /\ True)})
+  = h (ghost_vptr r)
